Coq Developments/msci/GV_Infrastructure.v
@@ -1,0 +1,186 @@
+(** Beginning of the file for GV infrastructure. *)
+Require Import Metatheory Coq.Program.Tactics Program.Equality.
+Require Import GV_Definitions.
+
+Set Implicit Arguments.
+
+Lemma eq_kind_dec: forall (x y : kind), sumbool (x = y) (x <> y).
+Proof. decide equality. Qed.
+
+Hint Resolve eq_kind_dec.
+
+Instance EqDec_kind : @EqDec_eq kind.
+Proof. exact eq_kind_dec. Defined.
+
+(** Uses heterogeneous equality but I believe this to be sound. *)
+Lemma eq_typ_dec: forall {k} (x y : typ k),
+  sumbool (x = y) (x <> y).
+Proof. 
+  ii; generalize dependent y; dependent induction x
+  ; dependent destruction y; auto; try (by right; ii; discriminate).
+  - destruct (k == k0) as [KEQ|]
+    ; [symmetry in KEQ; subst
+      |right; ii; inversion H; inversion H2; congruence].
+    specialize (IHx1 y1); specialize (IHx2 y2); destruct IHx1; destruct IHx2
+    ; try (by right; ii; inversion H; repeat simpl_existT; congruence).
+    left; congruence.
+  - destruct (k == k0) as [KEQ|]
+    ; [symmetry in KEQ; subst
+      |right; ii; inversion H; inversion H2; congruence].
+    specialize (IHx1 y1); specialize (IHx2 y2); destruct IHx1; destruct IHx2
+    ; try (by right; ii; inversion H; repeat simpl_existT; congruence).
+    left; congruence.
+  - specialize (IHx1 y1); specialize (IHx2 y2); destruct IHx1; destruct IHx2
+    ; try (by right; ii; inversion H; repeat simpl_existT; congruence).
+    left; congruence.
+  - specialize (IHx1 y1); specialize (IHx2 y2); destruct IHx1; destruct IHx2
+    ; try (by right; ii; inversion H; repeat simpl_existT; congruence).
+    left; congruence.
+  - destruct (kt == kt0) as [KEQ|]
+    ; [symmetry in KEQ; subst
+      |right; ii; inversion H; inversion H2; congruence].
+    destruct (ku == ku0) as [KEQ|]
+    ; [symmetry in KEQ; subst
+      |right; ii; inversion H; inversion H2; congruence].
+    specialize (IHx1 y1); specialize (IHx2 y2); destruct IHx1; destruct IHx2
+    ; try (by right; ii; inversion H; repeat simpl_existT; congruence).
+    left; congruence.
+  - destruct (kt == kt0) as [KEQ|]
+    ; [symmetry in KEQ; subst
+      |right; ii; inversion H; inversion H2; congruence].
+    destruct (ku == ku0) as [KEQ|]
+    ; [symmetry in KEQ; subst
+      |right; ii; inversion H; inversion H2; congruence].
+    specialize (IHx1 y1); specialize (IHx2 y2); destruct IHx1; destruct IHx2
+    ; try (by right; ii; inversion H; repeat simpl_existT; congruence).
+    left; congruence.
+  - destruct (kt == kt0) as [KEQ|]
+    ; [symmetry in KEQ; subst
+      |right; ii; inversion H; inversion H2; congruence].
+    destruct (ku == ku0) as [KEQ|]
+    ; [symmetry in KEQ; subst
+      |right; ii; inversion H; inversion H2; congruence].
+    specialize (IHx1 y1); specialize (IHx2 y2); destruct IHx1; destruct IHx2
+    ; try (by right; ii; inversion H; repeat simpl_existT; congruence).
+    left; congruence.
+Qed.
+
+Instance EqDec_typ {k}: @EqDec_eq (typ k).
+Proof. exact eq_typ_dec. Defined.
+
+(** Following ``Engineering Formal Metatheory'', we need some properties
+    regarding opening and substitution w.r.t locally closed terms.
+*)
+Section GVBasicSubstOpenProperties.
+
+  (* try to solve some proof obligations related to vars. *)
+  Ltac vcrush :=
+    destruct_all var; des; ss; des; try easy.
+
+  Lemma open_rec_same :
+    forall t j v i u
+           (NEQ: i <> j)
+           (EQ: {i ~> u}({j ~> v} t) = {j ~> v} t),
+      {i ~> u} t = t.
+  Proof.
+    induction t; ii; ss; auto
+    ; try (by f_equal; inversion EQ; firstorder)
+    ; des; auto.
+    - subst n; exfalso; auto.
+    - subst n; ss; destruct (i == i); auto; []; exfalso; auto.
+  Qed.
+
+  Lemma lc_no_bvar:
+    forall t u k
+           (LC: lc t),
+      {k ~> u}t = t.
+  Proof.
+    ii; generalize dependent k; induction LC; s; ii; f_equal; auto
+    ; try (by unfold open in *; pick fresh x for L
+           ; apply open_rec_same with (j := 0)(v := x); auto).
+    Case "let".
+      unfold open in *; pick fresh x for L; pick fresh y for L'.
+      apply open_rec_same with (j := 0)(v := y); auto.
+      apply open_rec_same with (j := 1)(v := x); auto.
+  Qed.
+
+  Lemma lc_open_subst:
+    forall t u (x y: atom) k
+           (NEQ: x <> y)
+           (LCU: lc u),
+      {k ~> y} ([x ~> u]t) = [x ~> u]({k ~> y} t).
+  Proof.
+    ii; unfold open; generalize dependent k.
+    induction t; ii; f_equal; auto.
+    vcrush; auto using lc_no_bvar.
+  Qed.
+
+  Lemma subst_eq_var:
+    forall (x : atom) u,
+      [x ~> u]x = u.
+  Proof.
+    ii; des; auto.
+  Qed.
+
+  Lemma subst_neq_var :
+    forall (x y : atom) u,
+      y <> x -> [x ~> u]y = y.
+  Proof.
+    ii; des; auto; []; exfalso; auto.
+  Qed.
+
+  Lemma subst_open_rec :
+    forall t1 t2 u (x : atom) k,
+      lc u ->
+      [x ~> u] ({k ~> t2} t1) = {k ~> [x ~> u] t2} ([x ~> u] t1).
+  Proof.
+    induction t1; ii; try (by f_equal; eauto).
+    vcrush; symmetry; auto using lc_no_bvar.
+  Qed.
+
+  Lemma subst_open_var :
+    forall (x y : atom) u t
+           (NEQ: y <> x)
+           (LC: lc u),
+      open ([x ~> u] t) y = [x ~> u] (open t y).
+  Proof.
+    ii; unfold open; auto using lc_open_subst.
+  Qed.
+
+  Lemma subst_intro :
+    forall (x : atom) u t
+           (NIN: x `notin` (GVFV t)),
+      open t u = [x ~> u](open t x).
+  Proof.
+    ii; unfold open; generalize 0.
+    induction t; intros bv; ss; try (solve [f_equal; eauto]).
+    - vcrush; apply notin_singleton_1 in NIN; tryfalse. 
+    - destruct_all var; f_equal; eauto.
+  Qed.
+
+  Lemma subst_lc :
+    forall t u x
+           (LCT: lc t)
+           (LC: lc u),
+      lc ([ x ~> u ] t).
+  Proof.
+    ii; induction LCT; simpl; auto.
+    Case "lc_id".
+      ss; destruct (x == x0); subst; eauto.
+    Case "lc_abs".
+      pick fresh y and apply lc_abs.
+      unfold open in *; rewrite lc_open_subst; auto.
+    Case "let".
+      (* TODO: tactic for introducing list of fresh variables. *)
+      apply lc_let with (L' := L `union` L' `union` singleton x)
+                          (L := L `union` L' `union` singleton x); ii; auto.
+      unfold open in *; rewrite !lc_open_subst; auto.
+    Case "case".
+      pick fresh y and apply lc_case; auto
+      ; by unfold open in *; rewrite lc_open_subst; auto.
+    Case "connect".
+      pick fresh y and apply lc_connect; unfold open in *
+      ; rewrite lc_open_subst; auto.
+  Qed.
+
+End GVBasicSubstOpenProperties.
