Coq Developments/msci/GV_Typing.v
@@ -1,0 +1,40 @@
+(** Beginning of the file for GV typing lemmas. *)
+Require Import Metatheory.
+Require Import GV_Definitions GV_Infrastructure.
+Set Implicit Arguments.
+
+Lemma elab_inl: forall (T: typ lin), ⟪T⟫ = inl T.
+Proof. auto. Qed.
+
+Lemma elab_inr: forall (T: typ un), ⟪T⟫ = inr T.
+Proof. auto. Qed.
+
+Lemma unlimited_env_typing:
+  forall Φ t (T: typ un)
+         (WT: Φ ⊢ t ∈ T),
+    un_env Φ.
+Proof.
+  ii; inversion WT; repeat simpl_existT; substs; auto; unfold un_env; i
+  ; simpl_env in *.
+  - rewrite elab_inr in *; destruct_in; substs; eauto.
+  - fsetdec.
+  - destruct_in. admit (* analyze_in x0 IN0 *). substs; eauto.
+  - destruct_in. admit (* analyze_in x IN0 *). admit (*analyze_in x IN1*).
+Admitted.
+
+Lemma typing_subst:
+  forall Φ Ψ k (T: typ k) (U: typ un) z t u
+         (WTT: Φ ++ (z ~ inr U) ++ Ψ ⊢ t ∈ T)
+         (WTU: Φ ⊢ u ∈ U),
+    Φ ++ Ψ ⊢ [z ~> u]t ∈ T.
+Proof.
+  ii; assert (UNENV: un_env Φ) by eauto using unlimited_env_typing.
+  induction WTT.
+Admitted.
+
+Lemma wt_tm_is_lc : forall Φ t k (T: typ k)
+    (WT: Φ ⊢ t ∈ T),
+  lc t.
+Proof.
+  ii; induction WT; eauto using subst_lc.
+Qed.
